AOS Project2

Adv Operating Systems/Project3/Cache.h
@@ -1,0 +1,16 @@
+#include <string>
+#include <iostream>
+
+using namespace std;
+
+class Cache {
+protected:
+    size_t cachesize;
+public:
+    Cache(size_t size):cachesize(size){};
+    virtual ~Cache(){};
+    virtual string* get(string url) {return NULL;};
+    virtual void put(string url, string page) {
+        cout<<url+" page cached"<<endl;
+    };
+};
