Adv Operating Systems/Project3/FIFOCache.cpp
@@ -1,0 +1,34 @@
+#include "FIFOCache.h"
+
+FIFOCache::FIFOCache(size_t size) {
+    cachesize = size;
+    currsize = 0;
+}
+
+string* FIFOCache::get(string url) {
+    map<string, string>::iterator it = this->mapTable.find(url);
+    if (it == mapTable.end())
+        return NULL;
+    else {
+        return &(it->second);
+    }
+}
+
+void FIFOCache::put(string url, string page) {
+    vector<string>::iterator it = find(order.begin(), order.end(), url);
+    if (it == order.end()) {
+        while (currsize + page.size() > cachesize) {
+            string oldurl = order.front();
+            order.erase(order.begin());
+            currsize = currsize - (mapTable[oldurl]).size();
+            mapTable.erase(oldurl);
+        }
+        currsize = currsize + page.size();                
+        order.push_back(url);
+    }
+
+    mapTable[url] = page;
+}
+
+void FIFOCache::updateOrder(string url) {
+}
