Adv Operating Systems/Project3/FIFOCache.h
@@ -1,0 +1,22 @@
+#include <string>
+#include <iostream>
+#include <map>
+#include <vector>
+#include <algorithm>
+
+using namespace std;
+
+class FIFOCache {
+protected:
+    size_t cachesize;
+    size_t currsize;
+public:
+    map<string, string> mapTable;
+    vector<string> order;
+    FIFOCache(size_t size);
+    ~FIFOCache(){};
+    string* get(string url);
+    void put(string url, string page);
+private:
+    void updateOrder(string url);
+};
