Adv Operating Systems/Project3/MAXSCache.cpp
@@ -1,0 +1,43 @@
+#include "MAXSCache.h"
+
+MAXSCache::MAXSCache(size_t size) {
+    cachesize = size;
+    currsize = 0;
+}
+
+string* MAXSCache::get(string url) {
+    map<string, string>::iterator it = this->mapTable.find(url);
+    if (it == mapTable.end())
+        return NULL;
+    else {
+        return &(it->second);
+    }
+}
+
+void MAXSCache::put(string url, string page) {
+    set<pair<int, string> >::iterator it = order.begin();
+    for (; it != order.end(); it++) {
+        if (it->second == url)
+            break;
+    }
+    if (it == order.end()) {
+        while (currsize + page.size() > cachesize) {
+            pair<int, string> oldurlpair = *(order.begin());
+            order.erase(order.begin());
+            currsize = currsize - (mapTable[oldurlpair.second]).size();
+            mapTable.erase(oldurlpair.second);
+        }
+        currsize = currsize + page.size();
+        order.insert(make_pair(page.size(), url));
+    }
+    mapTable[url] = page;
+    //this->updateOrder(url);
+}
+/*
+void MAXSCache::updateOrder(string url) {
+    sort(order.begin(), order.end(), cmp());
+}
+*/
+void MAXSCache::test() {
+    cout << "currsize is " << currsize << endl;
+}
