Adv Operating Systems/Project3/MAXSCache.h
@@ -1,0 +1,30 @@
+#include <string>
+#include <iostream>
+#include <map>
+#include <set>
+#include <algorithm>
+
+using namespace std;
+
+class MAXSCache {
+    // struct cmp
+    // {
+    //     bool operator ()(const pair<int, string> &a, const pair<int, string> &b)
+    //     {
+    //         return a.first > b.first;
+    //     }
+    // };
+protected:
+    size_t cachesize;
+    size_t currsize;
+public:
+    map<string, string> mapTable;
+    set<pair<int, string>, greater<pair<int, string> > > order;
+    MAXSCache(size_t size);
+    ~MAXSCache(){};
+    string* get(string url);
+    void put(string url, string page);
+    void test();
+private:
+    void updateOrder(string url);
+};
