Adv Operating Systems/Project3/RandomCache.cpp
@@ -1,0 +1,9 @@
+#include "RandomCache.h"
+
+RandomCache::RandomCache(size_t size) {
+    cacheSize = size;
+}
+
+RandomCache::~RandomCache() {
+    
+}
