Adv Operating Systems/Project3/RandomCache.h
@@ -1,0 +1,17 @@
+#include <string>
+#include <iostream>
+#include "Cache.h"
+
+using namespace std;
+
+class RandomCache : public Cache {
+protected:
+    
+public:
+    RandomCache(size_t size);
+    ~RandomCache(){};
+    string* get(string url) {return NULL;};
+    void put(string url, string page) {
+        cout<<url+" page cached"<<endl;
+    };
+};
