Adv Operating Systems/Project3/main.cpp
@@ -1,0 +1,30 @@
+#include <iostream>
+#include "FIFOCache.cpp"
+#include "LRUCache.cpp"
+#include "MAXSCache.cpp"
+
+int main(){
+    MAXSCache* fifoCache = new MAXSCache(50);
+    fifoCache->put("1", "abcd");
+    fifoCache->put("2", "secondStringTest");
+    fifoCache->put("2", "secondStringTest");
+    fifoCache->put("2", "hhhhh");
+    fifoCache->put("3", "longgeeeeeeeeeeehndnfcnsanannan");
+    fifoCache->put("1", "aaaa");
+    fifoCache->put("4", "sadfaffaaf");
+    fifoCache->put("5", "jnfdsjkafkj");
+    fifoCache->put("6", "jnfdsjkafkj");
+    fifoCache->put("7", "jnfdsjkafkj");
+
+    
+    map<string, string>::iterator it;
+    for (it = (fifoCache->mapTable).begin(); it != (fifoCache->mapTable).end(); it++) {
+        cout << it->first << " and " << it->second << endl;
+    }
+    cout << "The order is " << endl;
+    for (set<pair<int, string> >::iterator it = (fifoCache->order).begin(); it != (fifoCache->order).end(); it++) {
+        cout << (*it).second << " ";
+    }
+    cout << endl;
+    //fifoCache->test();
+}
